---
title: "The set N of Natural Numbers"
date: 2018-06-25T11:03:48+08:00
menuTitle: "Analysis"
volumes: ["1"]
layout: "note"
issue: 1

---


<!--more-->

<div class="latex-macros">
  {{< raw >}}
    $\newcommand{\br}{\\}$

    $\newcommand{\R}{\mathbb{R}}$
    $\newcommand{\Q}{\mathbb{Q}}$
    $\newcommand{\Z}{\mathbb{Z}}$
    $\newcommand{\N}{\mathbb{N}}$
    $\newcommand{\C}{\mathbb{C}}$
    $\newcommand{\P}{\mathbb{P}}$
    $\newcommand{\F}{\mathbb{F}}$
    $\newcommand{\L}{\mathcal{L}}$
    $\newcommand{\spa}[1]{\text{span}(#1)}$
    $\newcommand{\set}[1]{\{#1\}}$
    $\newcommand{\emptyset}{\varnothing}$
    $\newcommand{\otherwise}{\text{ otherwise }}$
    $\newcommand{\if}{\text{ if }}$
    $\newcommand{\proj}{\text{proj}}$
    $\newcommand{\union}{\cup}$
    $\newcommand{\intercept}{\cap}$
    $\newcommand{\abs}[1]{| #1 |}$
    $\newcommand{\norm}[1]{\left\lVert#1\right\rVert}$
    $\newcommand{\pare}[1]{\left\(#1\right\)}$
    $\newcommand{\t}[1]{\text{ #1 }}$
    $\newcommand{\head}{\text H}$
    $\newcommand{\tail}{\text T}$
    $\newcommand{\d}{\text d}$
    $\newcommand{\limu}[2]{\underset{#1 \to #2}\lim}$
    $\newcommand{\inv}[1]{{#1}^{-1}}$
    $\newcommand{\inner}[2]{\langle #1, #2 \rangle}$
    $\newcommand{\nullity}[1]{\text{nullity}(#1)}$
    $\newcommand{\rank}[1]{\text{rank}(#1)}$
    $\newcommand{\var}[1]{\text{var}(#1)}$
    $\newcommand{\tr}[1]{\text{tr}(#1)}$
    $\newcommand{\oto}{\text{ one-to-one }}$
    $\newcommand{\ot}{\text{ onto }}$
    $\newcommand{\Re}[1]{\text{Re}(#1)}$
    $\newcommand{\Im}[1]{\text{Im}(#1)}$


    $\newcommand{\Vcw}[2]{\begin{pmatrix} #1 \br #2 \end{pmatrix}}$
    $\newcommand{\Vce}[3]{\begin{pmatrix} #1 \br #2 \br #3 \end{pmatrix}}$
    $\newcommand{\Vcr}[4]{\begin{pmatrix} #1 \br #2 \br #3 \br #4 \end{pmatrix}}$
    $\newcommand{\Vct}[5]{\begin{pmatrix} #1 \br #2 \br #3 \br #4 \br #5 \end{pmatrix}}$
    $\newcommand{\Vcy}[6]{\begin{pmatrix} #1 \br #2 \br #3 \br #4 \br #5 \br #6 \end{pmatrix}}$
    $\newcommand{\Vcu}[7]{\begin{pmatrix} #1 \br #2 \br #3 \br #4 \br #5 \br #6 \br #7 \end{pmatrix}}$

    $\newcommand{\vcw}[2]{\begin{matrix} #1 \br #2 \end{matrix}}$
    $\newcommand{\vce}[3]{\begin{matrix} #1 \br #2 \br #3 \end{matrix}}$
    $\newcommand{\vcr}[4]{\begin{matrix} #1 \br #2 \br #3 \br #4 \end{matrix}}$
    $\newcommand{\vct}[5]{\begin{matrix} #1 \br #2 \br #3 \br #4 \br #5 \end{matrix}}$
    $\newcommand{\vcy}[6]{\begin{matrix} #1 \br #2 \br #3 \br #4 \br #5 \br #6 \end{matrix}}$
    $\newcommand{\vcu}[7]{\begin{matrix} #1 \br #2 \br #3 \br #4 \br #5 \br #6 \br #7 \end{matrix}}$

    $\newcommand{\Mqw}[2]{\begin{bmatrix} #1 & #2 \end{bmatrix}}$
    $\newcommand{\Mqe}[3]{\begin{bmatrix} #1 & #2 & #3 \end{bmatrix}}$
    $\newcommand{\Mqr}[4]{\begin{bmatrix} #1 & #2 & #3 & #4 \end{bmatrix}}$
    $\newcommand{\Mqt}[5]{\begin{bmatrix} #1 & #2 & #3 & #4 & #5 \end{bmatrix}}$

    $\newcommand{\Mwq}[2]{\begin{bmatrix} #1 \br #2 \end{bmatrix}}$
    $\newcommand{\Meq}[3]{\begin{bmatrix} #1 \br #2 \br #3 \end{bmatrix}}$
    $\newcommand{\Mrq}[4]{\begin{bmatrix} #1 \br #2 \br #3 \br #4 \end{bmatrix}}$
    $\newcommand{\Mtq}[5]{\begin{bmatrix} #1 \br #2 \br #3 \br #4 \br #5 \end{bmatrix}}$

    $\newcommand{\Mqw}[2]{\begin{bmatrix} #1 & #2 \end{bmatrix}}$
    $\newcommand{\Mwq}[2]{\begin{bmatrix} #1 \br #2 \end{bmatrix}}$
    $\newcommand{\Mww}[4]{\begin{bmatrix} #1 & #2 \br #3 & #4 \end{bmatrix}}$
    $\newcommand{\Mqe}[3]{\begin{bmatrix} #1 & #2 & #3 \end{bmatrix}}$
    $\newcommand{\Meq}[3]{\begin{bmatrix} #1 \br #2 \br #3 \end{bmatrix}}$
    $\newcommand{\Mwe}[6]{\begin{bmatrix} #1 & #2 & #3\br #4 & #5 & #6 \end{bmatrix}}$
    $\newcommand{\Mew}[6]{\begin{bmatrix} #1 & #2 \br #3 & #4 \br #5 & #6 \end{bmatrix}}$
    $\newcommand{\Mee}[9]{\begin{bmatrix} #1 & #2 & #3 \br #4 & #5 & #6 \br #7 & #8 & #9 \end{bmatrix}}$
  {{< /raw >}}
</div>

{{% properties name="Peano Axioms (Peano Postulates)" status="warning" %}}

**N1.** $1$ belongs to $\N $.

**N2.** If $n$ belongs to $\N $ then its successor $n + 1 $ belongs to $\N $.

**N3.** $1$ is not the successor of any element in $\N $.

**N4.** If $n $ and $m $ in $\N $ have the same successor, then $n = m $.

**N5.** A subset of $\N $ which contains $1$, and which contains $n + 1$ whenever it contains $n $, must equal $\N $. (Principal of Induction)

**N5'.** Every subset of $\N $ has a minimal element. (Well-orderedness)

<br>

From **N5'** we know the following:

**O1.** For $a,b \in \N, a \leq b $ or $b \leq a $.

**O2.** $a \leq b, b \leq a \implies a = b $.

**O3.** $a \leq b, b \leq c \implies a \leq c $.

<br>

**N1** - **N4**, **N5** $\iff$ **N1** - **N4**, **N5'**

{{% proof index="" name="" %}}

Let $X$ be a subset of $\N $, <br>
Show: **N1** - **N4**, **N5** $\implies$  $\forall x \in X, x \neq 1$ is a successor in $X $.

If $x \neq 1 $ and $x $ not a successor.

Let $X $ be a set of $\set{ 1 } \cup \set{ \text{all successors}} = \N$ by **N5**.

Then $x \in X , x \neq 1$ is CONTRADICTION; $x $ is a successor.

{{% /proof %}}

{{% /properties %}}

$P(n)$ statement (about $n$)

$S = \set{ n \mid P(n) \text{is true}}$ [Set of all $n$ s.t. $P(n)$ holds]
$P(1), P(n) \implies P(n + 1), S = \N, P(n)$ all $n $.

{{% example name="" %}}

$P(n) = 1 + 3 + 5 + ... + 2n - 1 =  n^2$

$P(1) = 1 = 1^2$

$P(2) = 1 + 3 = 4 = 2^2 $

Assume $P(n)$:

Then $1 + 3 + 5 + ... + 2n -1  = n^2 $

$1 + 3 + 5 + ... + 2n + 1 = n^2 + 2n + 1 $

$1 + 3 + 5 + ... + (2(n+1) - 1) = (n+1)^2 $

So $\P(n) \implies \P(n+1) $.

{{% /example %}}

{{% definition name="Complete (Strong) Induction" status="" %}}

$P(1)$

$P(m), \forall m \leq n \implies P(n+1)$

Then $P(n) \forall n $

Equivalent to **N5**.

{{% /definition %}}

{{% example name="" %}}

Try to prove that $N1 - N4, N5 \iff N1, ..., N4, N5' $

{{% /example %}}

{{% example name="" %}}

Every $n \in \N$ is a product of primes.

Let $P(n) $: $n $ is a product of primes.

Assume $P(m) $ is product of primes for all $m \leq n $.

For $n + 1$,

if $n+1 $ prime, then $n + 1$ is a product of prime.

if $n+1 $ not prime (composite), then $n + 1 = a \cdot b$ for some $a, b  \in \N$, $a,b  > 1$.

$\therefore$ by complete induction

$$a = p\_1, p\_2, ..., p\_{ k } $$

$$b = q\_1, q\_2, ..., q\_{ l } $$

$\therefore n + 1 = ab = p\_1 p\_2 ... p\_{ k } q\_1 q\_2 ... q\_{ l } $

$\therefore P(n + 1)$

Note: For $P(1)$, allow $1 $ to be a prime.

{{% /example %}}

{{% example name="" %}}

$P(n): \abs{ \sin(nx)} \leq n \abs{ \sin(x)} $

If $n = 1$, $\abs{ \sin (1 x)} \leq 1 \abs{ \sin x }$

Assume $P(n)$ consider

$\abs{ \sin ((n + 1) x)} = \abs{ \sin nx \cos x + \cos nx \sin x}$

$\abs{ a + b } \leq \abs{ a } + \abs{ b }$(triangle inequality)

$\therefore $

$\begin{align\*}
\abs{ \sin((n+1)x)} &\leq \abs{ \sin nx \cos x } + \abs{ \cos nx \sin x } \br
& \leq \abs{ \sin nx } \abs{ \cos x } + \abs{ \cos nx } \abs{ \sin x } \br
& \leq \abs{ \sin nx } \cdot 1 + 1 \cdot \abs{ \sin x } \br
& \leq n \abs{ \sin x } + \abs{  \sin x } = (n+1) \abs{ \sin x }
\end{align\*}$

$\therefore P(n + 1)$.

{{% /example %}}


